\documentclass{article}
\usepackage{iftex}
\usepackage{ifthen}
\usepackage{epsfig}
\usepackage[utf8]{inputenc}
\usepackage{xcolor}
\ifPDFTeX
\usepackage{newunicodechar}
  \makeatletter
    \def\doxynewunicodechar#1#2{%
    \@tempswafalse
    \edef\nuc@tempa{\detokenize{#1}}%
    \if\relax\nuc@tempa\relax
      \nuc@emptyargerr
    \else
      \edef\@tempb{\expandafter\@car\nuc@tempa\@nil}%
      \nuc@check
      \if@tempswa
        \@namedef{u8:\nuc@tempa}{#2}%
      \fi
    \fi
  }
  \makeatother
  \doxynewunicodechar{⁻}{${}^{-}$}% Superscript minus
  \doxynewunicodechar{²}{${}^{2}$}% Superscript two
  \doxynewunicodechar{³}{${}^{3}$}% Superscript three

\fi
\pagestyle{empty}
\begin{document}
$O(n)$
\pagebreak

\[ E(x) = (x + n)\;\mbox{mod}\; 26\]
\pagebreak

\[ D(x) = (x - n) \;\mbox{mod}\; 26\]
\pagebreak

$[a,b)$
\pagebreak

$[0,10]$
\pagebreak

$a$
\pagebreak

$b$
\pagebreak

$\text{size}\le10$
\pagebreak

$i^{th}$
\pagebreak

\[ E_{K}(M_{i}) = (M_{i} + K_{i})\;\mbox{mod}\; 26\]
\pagebreak

\[ D_{k}(C_{i}) = (C_{i} - K_{i} + 26)\;\mbox{mod}\; 26\]
\pagebreak

$K_{i}$
\pagebreak

$|key| < |text|$
\pagebreak

$(j + 1) \;\mbox{mod}\; |\mbox{key}|$
\pagebreak

$A {\oplus} 0 = A$
\pagebreak

$A {\oplus} A = 0$
\pagebreak

$ (A {\oplus} B) {\oplus} C = A {\oplus} (B {\oplus} C)$
\pagebreak

$ (B {\oplus} A) {\oplus} B = B {\oplus} 0 = B $
\pagebreak

$\oplus$
\pagebreak

$O(\log n)$
\pagebreak

$O(1)$
\pagebreak

$2^n\times n$
\pagebreak

$[i, j]$
\pagebreak

$i < 2^n$
\pagebreak

$j < n$
\pagebreak

$j$
\pagebreak

$(2^n - 1)^{\mbox{th}}$
\pagebreak

$i$
\pagebreak

$O(N \log N)$
\pagebreak

$N$
\pagebreak

$O(\log N)$
\pagebreak

\begin{eqnarray*}
x &=& R\left[ (1-k) \cos (t) + l\cdot k\cdot\cos \left(\frac{1-k}{k}t\right)
\right]\\
y &=& R\left[ (1-k) \sin (t) - l\cdot k\cdot\sin \left(\frac{1-k}{k}t\right)
\right] \end{eqnarray*}
\pagebreak

$R$
\pagebreak

$=1$
\pagebreak

$l=\frac{\rho}{r}$
\pagebreak

$0\le l\le1$
\pagebreak

$\rho$
\pagebreak

$r$
\pagebreak

$k=\frac{r}{R}$
\pagebreak

$0<k<1$
\pagebreak

$t$
\pagebreak

\[ f\left(x_0,x_1,x_2,\ldots\right) =
\sum_j x_jw_j+\theta
\]
\pagebreak

$x_j$
\pagebreak

$w_j$
\pagebreak

$\theta$
\pagebreak

$y$
\pagebreak

$x=y$
\pagebreak

$x+3y=-1$
\pagebreak

$x^2+y^2+z^2=r^2=1$
\pagebreak

$r^2<1$
\pagebreak

$1\times10^{-5}$
\pagebreak

\[
f(x) = \begin{cases}
-1 & \forall x \le 0\\
 1 & \forall x > 0
\end{cases}
\]
\pagebreak

$[a,b]$
\pagebreak

$(0,5, 0.5, 0.5)$
\pagebreak

$(0,5,-0.5, -0.5)$
\pagebreak

$(-0,5, 0.5, 0.5)$
\pagebreak

$(-0,5,-0.5, -0.5)$
\pagebreak

$0<\alpha\le1$
\pagebreak

\begin{eqnarray*}
r &\in& [1-\delta r, 1+\delta r)\\
\theta &\in& [0, 2\pi)\\
x &=& r\cos\theta\\
y &=& r\sin\theta
\end{eqnarray*}
\pagebreak

\begin{eqnarray*}
\delta r &=& 0.2\\
\delta x &\in& [-\delta r, \delta r)\\
\delta y &\in& [-\delta r, \delta r)\\
\theta &\in& [0, \pi)\\
x &=& \delta x + \cos\theta\\
y &=& \delta y + \frac{\sin(2\theta)}{2}
\end{eqnarray*}
\pagebreak

${0.5, 0.5, 0.5}$
\pagebreak

${0.5, 0.5, -0.5}$
\pagebreak

${0.5, -0.5, 0.5}$
\pagebreak

${0.5, -0.5, -0.5}$
\pagebreak

${-0.5, 0.5, 0.5}$
\pagebreak

${-0.5, 0.5, -0.5}$
\pagebreak

${-0.5, -0.5, 0.5}$
\pagebreak

${-0.5, -0.5, -0.5}$
\pagebreak

\[\beta = \left(X^TXX^T\right)Y\]
\pagebreak

\[y_{\text{row}=i} = \sum_{j=\text{columns}}\beta_j\cdot X_{i,j}\]
\pagebreak

$s(n)$
\pagebreak

\[
     s(n) = \sum_{d|n, d\neq n}d.
\]
\pagebreak

$s(18) = 1 + 2 + 3 + 6 + 9 = 21 $
\pagebreak

$a^b$
\pagebreak

$O(\log(b))$
\pagebreak

$O(b)$
\pagebreak

\begin{eqnarray*}
2^{10_d} &=& 2^{1010_b} = 2^8 * 2^2\\
2^1 &=& 2\\
2^2 &=& (2^1)^2 = 2^2 = 4\\
2^4 &=& (2^2)^2 = 4^2 = 16\\
2^8 &=& (2^4)^2 = 16^2 = 256\\
\end{eqnarray*}
\pagebreak

$2^8$
\pagebreak

$2^2$
\pagebreak

$2^1$
\pagebreak

$2^4$
\pagebreak

$O(\log(n))$
\pagebreak

$ \sqrt{z \bar{z}} $
\pagebreak

$ z $
\pagebreak

$n!!$
\pagebreak

\[\phi(n) =
\phi\left({p_1}^{a_1}\right)\cdot\phi\left({p_2}^{a_2}\right)\ldots\]
\pagebreak

$p_1$
\pagebreak

$p_2$
\pagebreak

$\ldots$
\pagebreak

$\phi(n) = n-1$
\pagebreak

$\phi(n^k) = n^k - n^{k-1}$
\pagebreak

$\phi(a,b) = \phi(a)\cdot\phi(b)$
\pagebreak

\[\phi(n) =
n\cdot\left(1-\frac{1}{p_1}\right)\cdot\left(1-\frac{1}{p_2}\right)\cdots\]
\pagebreak

$O\left(\sqrt{n}\right)$
\pagebreak

$\phi(100) = 40$
\pagebreak

$\phi(1) = 1$
\pagebreak

$\phi(17501) = 15120$
\pagebreak

$\phi(1420) = 560$
\pagebreak

\[\text{gcd}(a, b) = a \times x + b \times y \]
\pagebreak

\[r_0,\,r = r,\, r_0 - \text{quotient}\times r\]
\pagebreak

\[n! = n\times(n-1)\times(n-2)\times(n-3)\times\ldots\times3\times2\times1
      = n\times(n-1)!\]
\pagebreak

$5! = 5\times4! = 5\times4\times3\times2\times1 = 120$
\pagebreak

$O(logN)$
\pagebreak

$a^b = a^\frac{b}{2} \cdot a^\frac{b}{2} = {a^\frac{b}{2}}^2$
\pagebreak

$a^b = a^\frac{b-1}{2}
 \cdot a^\frac{b-1}{2} \cdot a = {a^\frac{b-1}{2}}^2 \cdot a$
\pagebreak

\[\text{fib}(n) = \text{fib}(n-1) + \text{fib}(n-2)\]
\pagebreak

$O(n\log n)$
\pagebreak

\[f(n)=f(n-1)+f(n-2)\]
\pagebreak

$\mathrm{F}(n) +
\mathrm{F}(n+1) + .. + \mathrm{F}(m)$
\pagebreak

$\mathrm{F}(n) + \mathrm{F}(n+1) + .. + \mathrm{F}(m)$
\pagebreak

$\mathrm{F}(i)$
\pagebreak

$\gcd(a, b, c)$
\pagebreak

$\gcd(\gcd(a, b), c)$
\pagebreak

$4! = 4\times3! = 4\times3\times2\times1 = 24$
\pagebreak

$\mathrm{LCM}(1,n) +
\mathrm{LCM}(2,n) + \ldots + \mathrm{LCM}(n,n)$
\pagebreak

$\mathrm{LCM}(i,n)$
\pagebreak

\[ \sum\mathrm{LCM}(i, n) = \frac{1}{2} \left[\left(\sum (d *
\mathrm{ETF}(d)) + 1\right) * n\right] \]
\pagebreak

$a^{n} \equiv r \mod{m}$
\pagebreak

$n$
\pagebreak

$m = mod
$
\pagebreak

$d \cdot 2^r = n - 1$
\pagebreak

$n = num$
\pagebreak

$r \geq 1$
\pagebreak

$num = 2^r \cdot d + 1$
\pagebreak

\[ϕ(m) = m-1\]
\pagebreak

$m$
\pagebreak

\begin{eqnarray*}
  a \cdot x &≡& 1 \;\text{mod}\; m\\
  x &≡& a^{-1} \;\text{mod}\; m
 \end{eqnarray*}
\pagebreak

\[
 a^{ϕ(m)} ≡ 1 \;\text{mod}\; m
 \]
\pagebreak

$a^{ϕ(m)} ≡ 1 \;\text{mod}\; m$
\pagebreak

$ϕ(m) = m-1$
\pagebreak

$a^{m-1} ≡ 1 \;\text{mod}\; m$
\pagebreak

$a^{-1}$
\pagebreak

\begin{eqnarray*}
 a^{m-1} \cdot a^{-1} &≡& a^{-1} \;\text{mod}\; m\\
 a^{m-2} &≡&  a^{-1} \;\text{mod}\; m
 \end{eqnarray*}
\pagebreak

$O(\log m)$
\pagebreak

$a^{-1} \;\text{mod}\; m$
\pagebreak

$a^{m-2} \;\text{mod}\; m$
\pagebreak

$3^5 \;\text{mod}\; 7 = 243 \;\text{mod}\; 7 = 5$
\pagebreak

$3^{-1} \;\text{mod}\; 7 = 5$
\pagebreak

$3 \times 5  \;\text{mod}\; 7 = 1 \;\text{mod}\; 7$
\pagebreak

$a\times a^{-1} = 1$
\pagebreak

$O(\sqrt{m})$
\pagebreak

$ \binom{n}{r} = \frac{n!}{r! (n-r)!} $
\pagebreak

$ \binom{n}{r} $
\pagebreak

$ \frac{n!}{r! (n-r)!} = \frac{(n - r + 1) \times \cdots \times n}{1 \times
\cdots \times r} $
\pagebreak

$ n $
\pagebreak

$ r $
\pagebreak

$N = p_1^{e_1} \times p_2^{e_2} \times\cdots\times p_k^{e_k}$
\pagebreak

$p_1,\, p_2,\, \dots,\, p_k$
\pagebreak

$e_1,\, e_2,\, \dots,\, e_k$
\pagebreak

$p_1^{g_1}\times p_2^{g_2}\times\cdots\times p_k^{g_k}$
\pagebreak

$0\le g_i\le e_i$
\pagebreak

$1\le i\le k$
\pagebreak

$(e_1+1) \times (e_2+1)\times\cdots\times (e_k+1)$
\pagebreak

$g_i$
\pagebreak

$N = 36 = (3^2 \cdot 2^2)$
\pagebreak

$\mbox{number_of_positive_divisors}(36) = (2+1) \cdot (2+1) = 9$
\pagebreak

$x^n$
\pagebreak

$1 <= x,\; n <= 10000$
\pagebreak

$O(N \cdot\log \log N)$
\pagebreak

$O(N)$
\pagebreak

$O(\log
N)$
\pagebreak

$x^2-a=0$
\pagebreak

$\pm\sqrt{a}$
\pagebreak

$f(x)=0$
\pagebreak

$f(a)<0$
\pagebreak

$f(b)>0$
\pagebreak

$(i+1)^\text{th}$
\pagebreak

\[
x_{i+1} = \frac{a_i+b_i}{2}
\]
\pagebreak

$[a,x]$
\pagebreak

$x>0$
\pagebreak

$[x,b]$
\pagebreak

$x<0$
\pagebreak

$f(x)$
\pagebreak

$f(x)= (x-2)^2$
\pagebreak

$[1,5]$
\pagebreak

$f(x)= x^{\frac{1}{x}}$
\pagebreak

$[-2,10]$
\pagebreak

$e\approx 2.71828182845904509$
\pagebreak

$f(x)= \cos x$
\pagebreak

$[0,12]$
\pagebreak

$\pi\approx 3.14159265358979312$
\pagebreak

$x^4-1=0$
\pagebreak

$x^2+4=0$
\pagebreak

$0 \pm 2i$
\pagebreak

$0.015625x^3-1=0$
\pagebreak

$(4+0i),\,(-2\pm3.464i)$
\pagebreak

\[
x_{i+1} = \frac{a_i\cdot f(b_i) - b_i\cdot f(a_i)}{f(b_i) - f(a_i)}
\]
\pagebreak

\[
k=\frac{3-\sqrt{5}}{2} \approx 0.381966\ldots\]
\pagebreak

\[
x_{i+1} = x_i - \frac{f(x_i)}{f'(x_i)}
\]
\pagebreak

\[
f(x) = x^3 - 4x - 9
\]
\pagebreak

$f'(x)$
\pagebreak

\[
f'(x) = 3x^2 - 4
\]
\pagebreak

\begin{eqnarray*}
   \dot{u} &=& v\\
   \dot{v} &=& -\omega^2 u\\
   \omega &=& 1\\
   [x_0, u_0, v_0] &=& [0,1,0]\qquad\ldots\text{(initial values)}
   \end{eqnarray*}
\pagebreak

\begin{eqnarray*}
   u(x) &=& \cos(x)\\
   v(x) &=& -\sin(x)\\
   \end{eqnarray*}
\pagebreak

\[y_{n+1}=y_n + dx\cdot f\left(x_n,y_n\right)\]
\pagebreak

$x_n$
\pagebreak

$x_{n+1}$
\pagebreak

$y_n$
\pagebreak

$y_{n+1}$
\pagebreak

$f\left(x_n,y_n\right)$
\pagebreak

\[y_{n+1} = y_n + dx\, f\left(x_n+\frac{1}{2}dx,
y_n + \frac{1}{2}dx\,f\left(x_n,y_n\right)\right)\]
\pagebreak

$\vec{a}=\left[a_0,a_1,a_2,...,a_L\right]$
\pagebreak

$\vec{b}=\left[b_0,b_1,b_1,...,b_L\right]$
\pagebreak

$\vec{a}\cdot\vec{b}=\displaystyle\sum_{i=0}^L a_i\times b_i$
\pagebreak

$\vec{a}\cdot\vec{b}$
\pagebreak

$\left|\vec{a}\right|=\sqrt{\displaystyle\sum_{i=0}^L a_i^2}$
\pagebreak

$\left|\vec{a}\right|$
\pagebreak

$\vec{a}$
\pagebreak

$\vec{b}$
\pagebreak

\[\text{proj}_\vec{b}\vec{a}=\frac{\vec{a}\cdot\vec{b}}{\left|\vec{b}\right|^2}\vec{b}\]
\pagebreak

$A$
\pagebreak

\begin{eqnarray*}
  \text{given that}\quad A &=&
*\left[\mathbf{a}_1,\mathbf{a}_2,\ldots,\mathbf{a}_{N-1},\right]\\
  \text{where}\quad\mathbf{a}_i &=&
  \left[a_{0i},a_{1i},a_{2i},\ldots,a_{(M-1)i}\right]^T\quad\ldots\mbox{(column
  vectors)}\\
  \text{then}\quad\mathbf{u}_i &=& \mathbf{a}_i
*-\sum_{j=0}^{i-1}\text{proj}_{\mathbf{u}_j}\mathbf{a}_i\\
  \mathbf{e}_i &=&\frac{\mathbf{u}_i}{\left|\mathbf{u}_i\right|}\\
  Q &=& \begin{bmatrix}\mathbf{e}_0 & \mathbf{e}_1 & \mathbf{e}_2 & \dots &
  \mathbf{e}_{N-1}\end{bmatrix}\\
  R &=& \begin{bmatrix}\langle\mathbf{e}_0\,,\mathbf{a}_0\rangle &
  \langle\mathbf{e}_1\,,\mathbf{a}_1\rangle &
  \langle\mathbf{e}_2\,,\mathbf{a}_2\rangle & \dots \\
                   0 & \langle\mathbf{e}_1\,,\mathbf{a}_1\rangle &
  \langle\mathbf{e}_2\,,\mathbf{a}_2\rangle & \dots\\
                   0 & 0 & \langle\mathbf{e}_2\,,\mathbf{a}_2\rangle &
  \dots\\ \vdots & \vdots & \vdots & \ddots
       \end{bmatrix}\\
  \end{eqnarray*}
\pagebreak

\[\begin{bmatrix}
5 & 7\\
7 & 11
\end{bmatrix}\]
\pagebreak

\[\begin{bmatrix}
-4& 4& 2& 0& -3\\
4& -4& 4& -3& -1\\
2& 4& 4& 3& -3\\
0& -3& 3& -1&-1\\
-3& -1& -3& -3& 0
\end{bmatrix}\]
\pagebreak

$c$
\pagebreak

$A' = A - cI$
\pagebreak

$A'=QR$
\pagebreak

$A'_1 = RQ $
\pagebreak

$A_1 = A'_1 + cI$
\pagebreak

$A_1$
\pagebreak

\[f(y) = 3y - \cos y -2\]
\pagebreak

\[f(y) = \frac{\cos y+2}{2}\]
\pagebreak

\[ C = K - 273.15 \]
\pagebreak

$a_i = b_i$
\pagebreak

$i <= k$
\pagebreak

$a_i = c_1 a_{i-1} + c_2 a_{i-2} + ... + c_k a_{i-k}$
\pagebreak

$i > k$
\pagebreak

$k=2$
\pagebreak

$b_1 = 1,\; b_2=1$
\pagebreak

$c_1 = 1,\; c_2=1$
\pagebreak

$a = \begin{bmatrix}0& 1& 1& 2& \ldots\end{bmatrix}$
\pagebreak

$10^{18}$
\pagebreak

$T^{n-1}$
\pagebreak

$\times$
\pagebreak

$p=n$
\pagebreak

$n^\text{th}$
\pagebreak

$6k\pm1$
\pagebreak

$A\equiv(x_1,y_1)$
\pagebreak

$B\equiv(x_2,y_2)$
\pagebreak

\[d=\sqrt{\left(x_1-x_2\right)^2+\left(y_1-y_2\right)^2}\]
\pagebreak

$a,\,b,\,c$
\pagebreak

$s=\displaystyle\frac{a+b+c}{2}$
\pagebreak

\[A=\sqrt{s(s-a)(s-b)(s-c)}\]
\pagebreak

$\frac{m\times n}{2}$
\pagebreak

$P(A|B)$
\pagebreak

$P(B|A)$
\pagebreak

$P(A)$
\pagebreak

$P(B)$
\pagebreak

$\mu=np$
\pagebreak

$\sigma^2 = n\cdot p\cdot (1-p)$
\pagebreak

$\sigma = \sqrt{\sigma^2} = \sqrt{n\cdot p\cdot (1-p)}$
\pagebreak

$\displaystyle {n\choose r} =
\frac{n!}{r!(n-r)!} = \frac{n\times(n-1)\times(n-2)\times\cdots(n-r)}{r!}
$
\pagebreak

$\displaystyle P(n,p,x) = {n\choose x} p^x (1-p)^{n-x}$
\pagebreak

$\displaystyle \left.P(n,p)\right|_{x_0}^{x_1} =
\sum_{i=x_0}^{x_1} P(i)
=\sum_{i=x_0}^{x_1} {n\choose i} p^i (1-p)^{n-i}$
\pagebreak

\[p(\mu,x) = \frac{\mu^x e^{-\mu}}{x!}\]
\pagebreak

\[P = \sum_i p(\mu,i)\]
\pagebreak

\begin{bmatrix}40 &30 &20 &50 &10\end{bmatrix}
\pagebreak

\begin{bmatrix}30 &40 &20 &50 &10\end{bmatrix}
\pagebreak

\begin{bmatrix}20 &30 &40 &50 &10\end{bmatrix}
\pagebreak

\begin{bmatrix}10 &20 &30 &40 &50\end{bmatrix}
\pagebreak

$O(n^2)$
\pagebreak

$O(n \log(n))$
\pagebreak

\begin{bmatrix}4 &3 &2 &5 &1\end{bmatrix}
\pagebreak

\begin{bmatrix}3 &4 &2 &5 &1\end{bmatrix}
\pagebreak

\begin{bmatrix}2 &3 &4 &5 &1\end{bmatrix}
\pagebreak

\begin{bmatrix}1 &2 &3 &4 &5\end{bmatrix}
\pagebreak

$O(n+N)$
\pagebreak

$arr[l\ldots i]$
\pagebreak

$arr[(i+1)\ldots (j-1)]$
\pagebreak

$arr[j\ldots r]$
\pagebreak

$O(nlogn)$
\pagebreak

\end{document}
